% TeX_root = ../main.tex

\marginnote{\scriptsize 04/03/2025 }

\section{Tensor Product of Normed Spaces}

\subsection{Few Facts}

Suppose $T : X \to X^\prime$ and $S: Y \to Y^\prime$ are linear. Then
there exist a unique linear map $T \otimes S : X \otimes Y \to
X^\prime \otimes Y^\prime$, such that
\begin{align*}
  (T \otimes S)(x \otimes y) = T(x) \otimes S(y)
\end{align*}

\begin{lemma}
  \label{lem:13}
  Let $x_1 , x_2 , \ldots , x_n \in X$, and $y_1 , y_2 , \ldots , y_n
  \in Y$. Then the following are equivalent
  \begin{enumerate}[label=(\arabic*)]
    \item $\sum_{i = 1}^{n} x_i \otimes y_i = 0$
    \item $\sum_{i = 1}^{n} \phi(x_i) \psi(y_i) = 0$ for all $\phi \in
      X^\dagger, \sigma \in Y^\dagger$
    \item $\sum_{i = 1}^{n} \psi(y_i) x_i = 0$
    \item $\sum_{i = 1}^{n} \phi(y_i) x_i = 0$
  \end{enumerate}
  where $X^\dagger$ is the collection of all linear functionals of
  $X$ and similarly $Y^\dagger$ for $Y$.
\end{lemma}
\begin{proof}
  Notice that we only need to prove $2 \implies 1$, and the rest is
  trivial \textcolor{red}{verify}.
  Let $z = \sum_{j = 1}^{k} \sum_{i = 1}^{m} c_{ij}(e_i \otimes
  d_j)$, where $c_{ij} \in \mathbb{C}$, $e_i$, $ d_j$ are linearly
  independent in $X, Y$ respectively. For each $1 \le i_o, j_o \le m$ by
  Hahn-Banach theorem, there is a $\phi \in X^*, \psi \in Y^*$ such
  that $\phi(e_i) = \delta_{i, i_o}, \psi(d_j) = \delta_{j, j_o}$.
\end{proof}

\begin{definition}
  Define for every $z \in X \otimes Y$,
  \begin{align*}
    \|z\|_{\wedge} = \inf \Big \{ \sum_{i = 1}^{n} \|x_i\|\|y_i\| \ : \  z =
    \sum_{i = 1}^{n} x_i \otimes y_i \Big \}
  \end{align*}
\end{definition}
\begin{proof}
  Scalar product comes out easily. \textcolor{red}{See that tringle
  inequality might also be satisfied}.

  Suppose $\|z\|_{\wedge} = 0$. Let $ \varepsilon > 0$ be given. Then there
  exists $x_1 , x_2 , \ldots , x_n \in X$, $y_1 , y_2 , \ldots , y_n
  \in Y$ such that $z = \sum_{i = 1}^{n} x_i \otimes y_i$, and
  \begin{align*}
    \sum_{i = 1}^{n} \|x_i\|\|y_i\| < \varepsilon
  \end{align*}
  Let $\phi \in X^\dagger$ with $\|\phi\| = 1$. Then
  \begin{align*}
    \Big \| \sum_{i = 1}^{n} \phi(x_i) y_i \Big \| < \varepsilon
  \end{align*}
  Then similarly for any $\psi \in Y^\dagger$, with $\|\psi\| = 1$, we get
  \begin{align*}
    \big|(\phi \otimes \psi)(z)\big| = \Big \|\sum_{i = 1}^{n}
    \phi(x_i) \psi(y_i) \Big \| < \varepsilon
  \end{align*}
  Notice that $\phi \otimes \psi \in (X \otimes Y)^\dagger$ since
  $\mathbb{C} \otimes \mathbb{C} = \mathbb{C}$.
  By appropriate rotation on each $x_i, y_i$, the above inequality becomes
  \begin{align*}
    \sum_{i = 1}^{n} |\phi(x_i)||\psi(y_i)| < \varepsilon
  \end{align*}
  Now by the \autoref{lem:13}, we are done.
\end{proof}

\begin{exercise}
  Show that
  \begin{align*}
    \|x \otimes y\|_{\wedge} = \|x\|\|y\|
  \end{align*}
\end{exercise}
